src/Bedrock/Curve/BN256Curve_G1_WiredSpecs.v
@@ -70,287 +70,55 @@ Local Lemma feval_wbw_def :
   forall ws, feval ws = F.of_Z M_pos (eval (from_mont (toZ ws))).
 Proof. reflexivity. Qed.
 
-Local Definition feval_toZ         := feval_toZ         feval_wbw_def.
-Local Definition feval_mul_bridge  := feval_mul_bridge  feval_wbw_def.
-Local Definition feval_add_bridge  := feval_add_bridge  feval_wbw_def.
-Local Definition feval_sub_bridge  := feval_sub_bridge  feval_wbw_def.
-Local Definition feval_square_bridge := feval_square_bridge feval_wbw_def.
-Local Definition feval_opp_bridge  := feval_opp_bridge  feval_wbw_def.
-(* [Z_opp_mod] is now available unqualified from the functor import. *)
+Require Import Bedrock.Curve.WbwMontgomeryG1_Transports.
 
-(** ** Transport lemmas -- proved via FElem bridge *)
+(** For WBW curves, [bounded_by tight_bounds], [bounded_by loose_bounds]
+    and [WordByWordMontgomery.valid] coincide definitionally. *)
+Local Lemma tight_of_valid :
+  forall ws, WordByWordMontgomery.valid bw n m (toZ ws) ->
+             bounded_by tight_bounds ws.
+Proof. intros ws H; exact H. Qed.
+Local Lemma valid_of_tight :
+  forall ws, bounded_by tight_bounds ws ->
+             WordByWordMontgomery.valid bw n m (toZ ws).
+Proof. intros ws H; exact H. Qed.
+Local Lemma valid_of_loose :
+  forall ws, bounded_by loose_bounds ws ->
+             WordByWordMontgomery.valid bw n m (toZ ws).
+Proof. intros ws H; exact H. Qed.
+Local Lemma loose_of_valid :
+  forall ws, WordByWordMontgomery.valid bw n m (toZ ws) ->
+             bounded_by loose_bounds ws.
+Proof. intros ws H; exact H. Qed.
 
-Lemma bn256_mul_bignum_correct :
+(** ** Transport lemmas -- via shared transport functor. *)
+
+Definition bn256_mul_bignum_correct :
   forall functions,
     spec_of_BinOp bin_mul (field_representation:=bn256_frep) functions ->
-    spec_of_bn256_mul_bignum functions.
-Proof.
-  intros functions Hfelem.
-  intros wsx wsy old_out px py pout tr m0 Rx Ry Rout.
-  intros Hvalx Hvaly Hlenout Hsepx Hsepy Hsepout.
-  pose proof (Bignum_length _ _ _ _ _ Hsepx) as Hlenx.
-  pose proof (Bignum_length _ _ _ _ _ Hsepy) as Hleny.
-  change 4%nat with felem_size_in_words in Hlenout, Hlenx, Hleny, Hsepx, Hsepy, Hsepout.
-  set (fx := exist _ wsx Hlenx : felem).
-  set (fy := exist _ wsy Hleny : felem).
-  set (fout := exist _ old_out Hlenout : felem).
-  seprewrite_in (Bignum_to_FElem px wsx Hlenx) Hsepx.
-  seprewrite_in (Bignum_to_FElem py wsy Hleny) Hsepy.
-  seprewrite_in (Bignum_to_FElem pout old_out Hlenout) Hsepout.
-  seprewrite_in (felem_to_bytes pout fout) Hsepout.
-  unfold spec_of_BinOp in Hfelem.
-  set (out_bs := ws2bs (Z.to_nat (bytes_per_word 64)) (felem_to_list fout)).
-  specialize (Hfelem pout px py fx fy out_bs Rout tr m0).
-  cbv [bin_mul bin_xbounds bin_ybounds bin_outbounds bin_model] in Hfelem.
-  assert (Hbdx : bounded_by loose_bounds (felem_to_list fx))
-    by (apply relax_bounds; exact Hvalx).
-  assert (Hbdy : bounded_by loose_bounds (felem_to_list fy))
-    by (apply relax_bounds; exact Hvaly).
-  assert (Hcall : call functions mul tr m0 [pout; px; py]
-    (fun (tr' : trace) (mem' : map.rep) (rets : list word.rep) =>
-       rets = [] /\ tr = tr' /\
-       (exists out0 : felem,
-          feval (felem_to_list out0) =
-          (feval (felem_to_list fx) * feval (felem_to_list fy))%F /\
-          bounded_by tight_bounds (felem_to_list out0) /\
-          (FElem pout out0 * Rout)%sep mem'))).
-  { apply Hfelem.
-    refine (conj Hbdx (conj Hbdy (conj _ (conj _ (conj _ _))))).
-    - exact (ws2bs_felem_length fout).
-    - exists Rx. exact Hsepx.
-    - exists Ry. exact Hsepy.
-    - exact Hsepout. }
-  eapply Proper_call; [ | exact Hcall].
-  clear Hcall Hfelem Hsepx Hsepy Hsepout Hbdx Hbdy.
-  intros tr' m' rets (Hrets & Htr & out0 & Hfeval_out & Hbd_out & Hsep_out).
-  split; [exact Htr|]. split; [exact Hrets|].
-  exists (felem_to_list out0).
-  split; [exact (proj2_sig out0)|].
-  split; [exact Hbd_out|].
-  split.
-  - seprewrite_in (FElem_iff_Bignum pout out0) Hsep_out.
-    change (proj1_sig out0) with (felem_to_list out0) in Hsep_out.
-    exact Hsep_out.
-  - apply (f_equal F.to_Z) in Hfeval_out.
-    rewrite F.to_Z_mul in Hfeval_out.
-    change (felem_to_list fx) with wsx in Hfeval_out.
-    change (felem_to_list fy) with wsy in Hfeval_out.
-    rewrite !feval_toZ in Hfeval_out.
-    change (Z.pos M_pos) with m in Hfeval_out.
-    rewrite Z.mul_mod_idemp_r in Hfeval_out by discriminate.
-    rewrite Zmod_mod.
-    exact Hfeval_out.
-Qed.
+    spec_of_bn256_mul_bignum functions
+  := mul_bignum_transport feval_wbw_def tight_of_valid valid_of_tight.
 
-Lemma bn256_add_bignum_correct :
+Definition bn256_add_bignum_correct :
   forall functions,
     spec_of_BinOp bin_add (field_representation:=bn256_frep) functions ->
-    spec_of_bn256_add_bignum functions.
-Proof.
-  intros functions Hfelem.
-  intros wsx wsy old_out px py pout tr m0 Rx Ry Rout.
-  intros Hvalx Hvaly Hlenout Hsepx Hsepy Hsepout.
-  pose proof (Bignum_length _ _ _ _ _ Hsepx) as Hlenx.
-  pose proof (Bignum_length _ _ _ _ _ Hsepy) as Hleny.
-  change 4%nat with felem_size_in_words in Hlenout, Hlenx, Hleny, Hsepx, Hsepy, Hsepout.
-  set (fx := exist _ wsx Hlenx : felem).
-  set (fy := exist _ wsy Hleny : felem).
-  set (fout := exist _ old_out Hlenout : felem).
-  seprewrite_in (Bignum_to_FElem px wsx Hlenx) Hsepx.
-  seprewrite_in (Bignum_to_FElem py wsy Hleny) Hsepy.
-  seprewrite_in (Bignum_to_FElem pout old_out Hlenout) Hsepout.
-  seprewrite_in (felem_to_bytes pout fout) Hsepout.
-  unfold spec_of_BinOp in Hfelem.
-  set (out_bs := ws2bs (Z.to_nat (bytes_per_word 64)) (felem_to_list fout)).
-  specialize (Hfelem pout px py fx fy out_bs Rout tr m0).
-  cbv [bin_add bin_xbounds bin_ybounds bin_outbounds bin_model] in Hfelem.
-  assert (Hcall : call functions add tr m0 [pout; px; py]
-    (fun (tr' : trace) (mem' : map.rep) (rets : list word.rep) =>
-       rets = [] /\ tr = tr' /\
-       (exists out0 : felem,
-          feval (felem_to_list out0) =
-          (feval (felem_to_list fx) + feval (felem_to_list fy))%F /\
-          bounded_by loose_bounds (felem_to_list out0) /\
-          (FElem pout out0 * Rout)%sep mem'))).
-  { apply Hfelem.
-    refine (conj Hvalx (conj Hvaly (conj _ (conj _ (conj _ _))))).
-    - exact (ws2bs_felem_length fout).
-    - exists Rx. exact Hsepx.
-    - exists Ry. exact Hsepy.
-    - exact Hsepout. }
-  eapply Proper_call; [ | exact Hcall].
-  clear Hcall Hfelem Hsepx Hsepy Hsepout.
-  intros tr' m' rets (Hrets & Htr & out0 & Hfeval_out & Hbd_out & Hsep_out).
-  split; [exact Htr|]. split; [exact Hrets|].
-  exists (felem_to_list out0).
-  split; [exact (proj2_sig out0)|].
-  split; [exact Hbd_out|].
-  split.
-  - seprewrite_in (FElem_iff_Bignum pout out0) Hsep_out.
-    change (proj1_sig out0) with (felem_to_list out0) in Hsep_out.
-    exact Hsep_out.
-  - apply (f_equal F.to_Z) in Hfeval_out.
-    rewrite F.to_Z_add in Hfeval_out.
-    change (felem_to_list fx) with wsx in Hfeval_out.
-    change (felem_to_list fy) with wsy in Hfeval_out.
-    rewrite !feval_toZ in Hfeval_out.
-    change (Z.pos M_pos) with m in Hfeval_out.
-    exact Hfeval_out.
-Qed.
+    spec_of_bn256_add_bignum functions
+  := add_bignum_transport feval_wbw_def tight_of_valid valid_of_loose.
 
-Lemma bn256_sub_bignum_correct :
+Definition bn256_sub_bignum_correct :
   forall functions,
     spec_of_BinOp bin_sub (field_representation:=bn256_frep) functions ->
-    spec_of_bn256_sub_bignum functions.
-Proof.
-  intros functions Hfelem.
-  intros wsx wsy old_out px py pout tr m0 Rx Ry Rout.
-  intros Hvalx Hvaly Hlenout Hsepx Hsepy Hsepout.
-  pose proof (Bignum_length _ _ _ _ _ Hsepx) as Hlenx.
-  pose proof (Bignum_length _ _ _ _ _ Hsepy) as Hleny.
-  change 4%nat with felem_size_in_words in Hlenout, Hlenx, Hleny, Hsepx, Hsepy, Hsepout.
-  set (fx := exist _ wsx Hlenx : felem).
-  set (fy := exist _ wsy Hleny : felem).
-  set (fout := exist _ old_out Hlenout : felem).
-  seprewrite_in (Bignum_to_FElem px wsx Hlenx) Hsepx.
-  seprewrite_in (Bignum_to_FElem py wsy Hleny) Hsepy.
-  seprewrite_in (Bignum_to_FElem pout old_out Hlenout) Hsepout.
-  seprewrite_in (felem_to_bytes pout fout) Hsepout.
-  unfold spec_of_BinOp in Hfelem.
-  set (out_bs := ws2bs (Z.to_nat (bytes_per_word 64)) (felem_to_list fout)).
-  specialize (Hfelem pout px py fx fy out_bs Rout tr m0).
-  cbv [bin_sub bin_xbounds bin_ybounds bin_outbounds bin_model] in Hfelem.
-  assert (Hcall : call functions sub tr m0 [pout; px; py]
-    (fun (tr' : trace) (mem' : map.rep) (rets : list word.rep) =>
-       rets = [] /\ tr = tr' /\
-       (exists out0 : felem,
-          feval (felem_to_list out0) =
-          (feval (felem_to_list fx) - feval (felem_to_list fy))%F /\
-          bounded_by loose_bounds (felem_to_list out0) /\
-          (FElem pout out0 * Rout)%sep mem'))).
-  { apply Hfelem.
-    refine (conj Hvalx (conj Hvaly (conj _ (conj _ (conj _ _))))).
-    - exact (ws2bs_felem_length fout).
-    - exists Rx. exact Hsepx.
-    - exists Ry. exact Hsepy.
-    - exact Hsepout. }
-  eapply Proper_call; [ | exact Hcall].
-  clear Hcall Hfelem Hsepx Hsepy Hsepout.
-  intros tr' m' rets (Hrets & Htr & out0 & Hfeval_out & Hbd_out & Hsep_out).
-  split; [exact Htr|]. split; [exact Hrets|].
-  exists (felem_to_list out0).
-  split; [exact (proj2_sig out0)|].
-  split; [exact Hbd_out|].
-  split.
-  - seprewrite_in (FElem_iff_Bignum pout out0) Hsep_out.
-    change (proj1_sig out0) with (felem_to_list out0) in Hsep_out.
-    exact Hsep_out.
-  - change (felem_to_list fx) with wsx in Hfeval_out.
-    change (felem_to_list fy) with wsy in Hfeval_out.
-    apply (feval_sub_bridge _ _ _ Hfeval_out).
-Qed.
+    spec_of_bn256_sub_bignum functions
+  := sub_bignum_transport feval_wbw_def tight_of_valid valid_of_loose.
 
-Lemma bn256_square_bignum_correct :
+Definition bn256_square_bignum_correct :
   forall functions,
     spec_of_UnOp un_square (field_representation:=bn256_frep) functions ->
-    spec_of_bn256_square_bignum functions.
-Proof.
-  intros functions Hfelem.
-  intros wsx old_out px pout tr m0 Rx Rout.
-  intros Hvalx Hlenout Hsepx Hsepout.
-  pose proof (Bignum_length _ _ _ _ _ Hsepx) as Hlenx.
-  change 4%nat with felem_size_in_words in Hlenout, Hlenx, Hsepx, Hsepout.
-  set (fx := exist _ wsx Hlenx : felem).
-  set (fout := exist _ old_out Hlenout : felem).
-  seprewrite_in (Bignum_to_FElem px wsx Hlenx) Hsepx.
-  seprewrite_in (Bignum_to_FElem pout old_out Hlenout) Hsepout.
-  seprewrite_in (felem_to_bytes pout fout) Hsepout.
-  unfold spec_of_UnOp in Hfelem.
-  set (out_bs := ws2bs (Z.to_nat (bytes_per_word 64)) (felem_to_list fout)).
-  specialize (Hfelem pout px fx out_bs Rout tr m0).
-  cbv [un_square un_xbounds un_outbounds un_model] in Hfelem.
-  assert (Hcall : call functions square tr m0 [pout; px]
-    (fun (tr' : trace) (mem' : map.rep) (rets : list word.rep) =>
-       rets = [] /\ tr = tr' /\
-       (exists out0 : felem,
-          feval (felem_to_list out0) =
-          F.pow (feval (felem_to_list fx)) 2 /\
-          bounded_by tight_bounds (felem_to_list out0) /\
-          (FElem pout out0 * Rout)%sep mem'))).
-  { apply Hfelem.
-    refine (conj Hvalx (conj _ (conj _ _))).
-    - exact (ws2bs_felem_length fout).
-    - exists Rx. exact Hsepx.
-    - exact Hsepout. }
-  eapply Proper_call; [ | exact Hcall].
-  clear Hcall Hfelem Hsepx Hsepout.
-  intros tr' m' rets (Hrets & Htr & out0 & Hfeval_out & Hbd_out & Hsep_out).
-  split; [exact Htr|]. split; [exact Hrets|].
-  exists (felem_to_list out0).
-  split; [exact (proj2_sig out0)|].
-  split; [exact Hbd_out|].
-  split.
-  - seprewrite_in (FElem_iff_Bignum pout out0) Hsep_out.
-    change (proj1_sig out0) with (felem_to_list out0) in Hsep_out.
-    exact Hsep_out.
-  - apply (f_equal F.to_Z) in Hfeval_out.
-    rewrite F.to_Z_pow in Hfeval_out.
-    change (felem_to_list fx) with wsx in Hfeval_out.
-    rewrite !feval_toZ in Hfeval_out.
-    simpl Z.of_N in Hfeval_out.
-    rewrite Z.pow_2_r in Hfeval_out.
-    change (Z.pos M_pos) with m in Hfeval_out.
-    exact Hfeval_out.
-Qed.
+    spec_of_bn256_square_bignum functions
+  := square_bignum_transport feval_wbw_def valid_of_tight loose_of_valid.
 
-Lemma bn256_opp_bignum_correct :
+Definition bn256_opp_bignum_correct :
   forall functions,
     spec_of_UnOp un_opp (field_representation:=bn256_frep) functions ->
-    spec_of_bn256_opp_bignum functions.
-Proof.
-  intros functions Hfelem.
-  intros wsx old_out px pout tr m0 Rx Rout.
-  intros Hvalx Hlenout Hsepx Hsepout.
-  pose proof (Bignum_length _ _ _ _ _ Hsepx) as Hlenx.
-  change 4%nat with felem_size_in_words in Hlenout, Hlenx, Hsepx, Hsepout.
-  set (fx := exist _ wsx Hlenx : felem).
-  set (fout := exist _ old_out Hlenout : felem).
-  seprewrite_in (Bignum_to_FElem px wsx Hlenx) Hsepx.
-  seprewrite_in (Bignum_to_FElem pout old_out Hlenout) Hsepout.
-  seprewrite_in (felem_to_bytes pout fout) Hsepout.
-  unfold spec_of_UnOp in Hfelem.
-  set (out_bs := ws2bs (Z.to_nat (bytes_per_word 64)) (felem_to_list fout)).
-  specialize (Hfelem pout px fx out_bs Rout tr m0).
-  cbv [un_opp un_xbounds un_outbounds un_model] in Hfelem.
-  assert (Hcall : call functions opp tr m0 [pout; px]
-    (fun (tr' : trace) (mem' : map.rep) (rets : list word.rep) =>
-       rets = [] /\ tr = tr' /\
-       (exists out0 : felem,
-          feval (felem_to_list out0) =
-          F.opp (feval (felem_to_list fx)) /\
-          bounded_by loose_bounds (felem_to_list out0) /\
-          (FElem pout out0 * Rout)%sep mem'))).
-  { apply Hfelem.
-    refine (conj Hvalx (conj _ (conj _ _))).
-    - exact (ws2bs_felem_length fout).
-    - exists Rx. exact Hsepx.
-    - exact Hsepout. }
-  eapply Proper_call; [ | exact Hcall].
-  clear Hcall Hfelem Hsepx Hsepout.
-  intros tr' m' rets (Hrets & Htr & out0 & Hfeval_out & Hbd_out & Hsep_out).
-  split; [exact Htr|]. split; [exact Hrets|].
-  exists (felem_to_list out0).
-  split; [exact (proj2_sig out0)|].
-  split; [exact Hbd_out|].
-  split.
-  - seprewrite_in (FElem_iff_Bignum pout out0) Hsep_out.
-    change (proj1_sig out0) with (felem_to_list out0) in Hsep_out.
-    exact Hsep_out.
-  - apply (f_equal F.to_Z) in Hfeval_out.
-    rewrite F.to_Z_opp in Hfeval_out.
-    change (felem_to_list fx) with wsx in Hfeval_out.
-    rewrite !feval_toZ in Hfeval_out.
-    change (Z.pos M_pos) with m in Hfeval_out.
-    (* H: -(a mod m) mod m; goal: (-a) mod m mod m *)
-    rewrite Z_opp_mod in Hfeval_out. rewrite Zmod_mod. exact Hfeval_out.
-Qed.
+    spec_of_bn256_opp_bignum functions
+  := opp_bignum_transport feval_wbw_def tight_of_valid valid_of_loose.
